# HW 11

### 5-1

$$
T = \frac{2\pi}{w} = 10^{-3}s\\
w_s > 2w_c\\
(1),(3),(4)可以恢复
$$

### 5-2

(1)
$$
x(t) = 2+cos(1000\pi t)+sin(3000\pi t)\\
奈奎斯特频率:6000\pi
$$
(3)
$$
x(t) = (\frac{sinw_ct}{\pi t})^2 = \frac{1-cos2w_ct}{2(\pi t)^2}\\
奈奎斯特频率:4w_c
$$
(5)
$$
x(t) = (\frac{sin1000\pi t}{\pi t})(\frac{sin2000\pi t}{\pi t})\\
奈奎斯特频率:6000\pi
$$

### 5-3

$$
x(t) = \sum_{k=0}^5(\frac{1}{2})^ksin(k\pi t)
$$

(1)
$$
w_s = 10\pi = 2w_M\\
会发生混叠
$$
(2)
$$
由于截止频率为5\pi\\
x_r(t) = sum_{k=0}^4(\frac{1}{2})^ksin(k\pi t)
$$

### 5-4

$$
x_r(t) = \sum x(nT)h(t-nT),x(t) = cos2\pi t,T = 0.2\\
x_r(t) = x_p(t) * h(t) = [\sum x(nT)\delta(t-nT)] * h(t)\\
 = \sum x(nT)h(t-nT)\\
X(jw) = \pi[\delta(w+2\pi)+\delta(w-2\pi)]\\
X_p(jw) = \frac{1}{T}\sum_{k=-∞}^∞ X(j(w-kw_s)),w_s = \frac{2\pi}{T}\\
X_p(jw) = 5\pi \sum [\delta(w+10k\pi+2\pi)+\delta(w+10k\pi-2\pi)]\\
H(jw) = 0.2Sa^2(0.1w)\\
X_r(jw) = X_p(jw)·H(jw) = \pi Sa^2(0.1w)\sum [\delta(w+10k\pi+2\pi)+\delta(w+10k\pi-2\pi)]
$$

### 5-5

$$
x_r(t) = \sum x(nT)\frac{Tw_c}{\pi}Sa(w_c(t-nT)),w_c = \frac{w_s}{2}\\证明x_r(kT) = x(kT)\\
证明:\\
w_s = \frac{2\pi}{T}\\
w_c = \frac{\pi}{T}\\
x_r(kT) = \sum_{n = -∞}^∞ x(nT)Sa(k\pi - n\pi)\\
当n = k时,Sa(k\pi - n\pi)  =1\\
=>x_r(kT) = x(kT)
$$

### 5-6

(1):$f(t) = x_1(t)+x_2(t)$

T = 1/600

(3):$f(t) = x_2(2t)$

T = 1/1200

(5):$f(t) = x_1(t)·x_2(t/3)$

T = 1/200

### 5-8
$$
A = T,w_b = w_2,T = \frac{2\pi}{w_2},w_a\in(w_2-w_1,w_1)
$$

### 5-12

$$
x_c(n·10^{-3})<-->1000X(1000jw)\\
x_d[n]<-->X(e^{jw})\\
X_c(jw) = 1000X_d(e^{1000jw})
$$

(1):$X_c(jw)为实函数$

(2):
$$
X_c(jw) = 1000X_d(e^{jw1000})<1\\
X_c(jw)<1
$$
(3):
$$
X_c(jw) = 1000X_d(e^{jw1000})=0,|w|\in[\frac{3}{4}\pi,\pi]\\
X_c(jw) = 0,|w>=750\pi|
$$
(4):
$$
X_c(jw) = 1000X_d(e^{jw1000}) = 1000X_d(e^{j(w-\pi)1000}) = X_c(j(w-1000\pi))\\
X_c(jw) = X_c(j(w-1000\pi))
$$

### 5-16

$$
X(e^{jw}) = \frac{1}{T}\sum X(j(w-2k\pi)/T)\\
 = 20·10^3 \sum X(j(w-2k\pi)·20·10^3)\\
 Y(e^{jw}) = X(e^{jw})·H(e^{jw})\\
 Y_c(jw) = TY(e^{jwT}),T = \frac{1}{20kHz}
$$

### 5-17



### 5-18

$$
Y(e^{jw})-\frac{1}{3}e^{-jw}Y(e^{jw}) = X(e^{jw})\\
H(e^{jw}) = \frac{1}{1-\frac{1}{3}e^{-jw}}\\
H(jw) = TH(e^{jwT}) = \frac{T}{1-\frac{1}{3}e^{-jwT}}
$$

### 5-19

$$
\frac{sin300\pi t - sin100\pi t}{2}
$$

### 5-21

$$
设x_1(t) = [x(t)`cos5wt]*h_1(t)\\
X_1(jw) = \frac{X(j(w-5w))+X(j(w+5w))}{2}·H_1(jw)\\
设x_2(t) = [x_1(t)·cos3wt]*h_2(t)\\
X_2(jw) = \frac{H_1(j(w-3w))+X_1(j(w+3w))}{2}·H_2(jw)
$$

### 5-26

(1)
$$
R(w) = cosw\\
h(t) = \frac{\delta(t-1)+\delta(t+1)}{2}
$$
(2)
$$
R(w) = \frac{1}{1+w^2}\\
h(t) = e^{-|t|}/2\\
I(w) = R(w)*(-\frac{1}{\pi w})
$$

(3)
$$
证明H(jw) = \frac{1}{j\pi}\int \frac{H(j\lambda)}{w-\lambda}d\lambda\\
H(jw) = R(w)+jI(W)\\
R(w) = \frac{1}{\pi}\int \frac{I(\lambda)}{w-\lambda}d\lambda = I(w)*\frac{1}{\pi w}\\
I(w) = -\frac{1}{\pi}\int \frac{R(\lambda)}{w-\lambda}d\lambda = R(w)*(-\frac{1}{\pi w})\\
H(jw) = \frac{1}{\pi}\int \frac{I(\lambda)}{w-\lambda}d\lambda-j\frac{1}{\pi}\int \frac{R(\lambda)}{w-\lambda}d\lambda\\
 = \frac{1}{j\pi}\int \frac{H(j\lambda)}{w-\lambda}d\lambda
$$


### 5-27

(1)
$$
x(t) = a(t)cosw_0t+b(t)sinw_0t\\
\widehat{x}(t) = x(t)*\frac{1}{\pi t} = \frac{1}{\pi}\int \frac{x(\tau)}{t-\tau}d\tau\\
\widehat{x}(t) = H[x(t)]
$$
(2)
$$
\widehat{x}(t) = H[x(t)]\\
瞬时包络:|a(t)| = \sqrt{x(t)^2+\widehat{x}(t)^2} = \sqrt{x(t)^2+H[x(t)]^2}\\
瞬时相位:\phi(t) = arctan\frac{\widehat{x}(t)}{x(t)}=arctan\frac{H[x(t)]}{x(t)}\\
瞬时频率:w(t) = \frac{d\phi(t)}{dt} = \frac{d(arctan\frac{H[x(t)]}{x(t)})}{dt}
$$

