### Problem 1

---

​	牛顿方法如下：
$$
p_n = p_{n-1}-\frac{f(p_{n-1})}{f'(p_{n-1})}
$$
当$p_0$ = -1时，$p_2$ = -0.999949236,不能取$p_0$=0,因为f'(0)=0

### Problem2

---
​	(Ⅰ)
$$
X_k = 2X_{k-1}-bX_{k-1}^2\\
X_{k-1} = \frac{\xi_{k-1}+1}{b}\\
=>X_{k} = \frac{1-\xi_{k-1}^2}{b}\\
\xi_k = \frac{\frac{1}{b}-x_k}{\frac{1}{b}}\\
\xi_k = \xi_{k-1}^2\\
也就是|\xi_{k+1}| = \xi_{k}^2
$$

​	（Ⅱ)
$$
X_k = 2X_{k-1}-bX_{k-1}^2\\
x_0∈(0,\frac{2}{b})\\
=>x_1∈(0,\frac{1}{b})\\
又有\frac{1}{b} = 2\frac{1}{b}-b(\frac{1}{b})^2\\
\frac{1}{b}是f(x)=2x-bx^2的不动点\\
g'(x)=(2x-bx^2-x)'=1-2bx\\
当x∈(0,\frac{1}{b})时，|g'(x)|<1,由fixed-point~theorem可知\\
f(x)收敛于\frac{1}{b}
$$

### problem3

---

​	a.
$$
F(x_1,x_2,x_3)=(f_1(x_1,x_2,x_3),f_2(x_1,x_2,x_3),f_3(x_1,x_2,x_3))\\
f_1(x_1,x_2,x_3)=3x_1-cos(x_2x_3)-\frac{1}{2}\\
f_2(x_1,x_2,x_3)=4x_1^2-625x_2^2+2x_2-1\\
f_3(x_1,x_2,x_3)=e^{-x_1x_2}+20x_3+\frac{10\pi-3}{3}\\
Jacobian~~matrix：\\
J(x_1,x_2,x_3)=
[\begin{matrix}
3&x_3sin(x_2x_3)&x_2sin(x_2x_3)\\
8x_1&-1250x_2+2&0\\
-x_2e^{-x_1x_2}&-x_1e^{-x_1x_2}&20
\end{matrix}]
\\
x^{(0)} = 0 ~~~F(x^{(0)}) = (-\frac{3}{2},-1,\frac{10\pi}{3})^t\\
J(x^{(0)})=
[\begin{matrix}
3&0&0\\
0&2&0\\
0&0&20
\end{matrix}]
\\
J^{x(0)}y^{(0)}=-F(x^{(0)})\\
y^{(0)}=(\frac{1}{2},\frac{1}{2},\frac{-1\pi}{6})^t\\
x^{(1)}=x^{(0)}+y^{(0)}=(\frac{1}{2},\frac{1}{2},\frac{-1\pi}{6})^t\\
类似迭代\\
解得y^{(1)} = (0.00546566,0.24923252,-0.00610098)\\
x^{(2)}= y^{(1)}+x^{(1)}\\
x^{(2)}=(0.50546566,0.74923252,-0.52969976)
$$
b.

​	
$$
F(x_1,x_2,x_3)=(f_1(x_1,x_2,x_3),f_2(x_1,x_2,x_3),f_3(x_1,x_2,x_3))\\
f_1(x_1,x_2,x_3)=x_1^2+x_2-37\\
f_2(x_1,x_2,x_3)=x_1-x_2^2-5\\
f_3(x_1,x_2,x_3)=x_1+x_2+x_3-3\\
J(x_1,x_2,x_3)=
[\begin{matrix}
2x_1&1&0\\
1&2x_2&0\\
1&1&1\\
\end{matrix}]\\
x^{(0)}=0~~~F(x^{(0)})=(-37,-5,-3)\\
J(x^{(0)}) = 
[\begin{matrix}
0&1&0\\
1&0&0\\
1&1&1\\
\end{matrix}]\\
J^{x(0)}y^{(0)}=-F(x^{(0)})\\
y^{(0)} = (5,37,-39)^t\\
x^{(1)} = x^{(0)}+y^{(0)}\\
x^{(1)} = (5,37,-39)^t\\
同理，解得y^{(1)}=(1.126835,-18.26835781,17.14152203)\\
x^{(2)}= y^{(1)}+x^{(1)}\\
x^{(2)} = (6.126835,18.73164219,14.14152203)
$$

### Problem 4

---



a.
$$
f_1(x_1,x_2,x_3)=15x_1+x_2^2-4x_3-13\\
f_2(x_1,x_2,x_3)=x_1^2+10x_2-x_3-11\\
f_3(x_1,x_2,x_3)=x_2^3-25x_3+22\\
x^{(0)}=0\\
F(x^{(0)})=(-13,-11,22)^t\\
J(x^{(0)}) = 
[\begin{matrix}
15&0&-4\\
0&10&-1\\
0&0&-25
\end{matrix}]\\
g(x)=f_1(x_1,x_2,x_3)^2+f_2(x_1,x_2,x_3)^2+f_3(x_1,x_2,x_3)^2\\
g(x^{(0)})=774\\
\nabla g(x)=2J(x)^tF(x)\\
\nabla g(^{(0)})=
[\begin{matrix}
-566\\
-264\\
-1100
\end{matrix}]\\
z_0=||\nabla g(x^{(0)})||_2=1264.931619\\
z=\frac{1}{z_0}\nabla g(x^{0})=(-0.4474550177,-0.2087069341,-0.8696122253)\\
取\alpha_1=0\\
g_1=g(x^{(0)}-\alpha_1z)=g(x^{(0)})=774\\
取\alpha_3=1\\
g_3=g(x^{(0)}-\alpha_3z)=186.431202\\
取\alpha_2=\alpha_3/2\\
g_2=g(x^{(0)}-\alpha_2z)=360.171324\\
Set~P(\alpha)=g_1+h_1\alpha+h_3\alpha(\alpha-\alpha_2)\\
h_1=(g_2-g_1)/\alpha_2\\
h_2=(g_3-g_2)/(\alpha_3-\alpha_2)\\
h_3=(h_2-h_1)/\alpha_3\\
由于要找到\alpha 使得P最小，求导\\
P'(\alpha)=0\\
=>\alpha=1.077364\\
x^{(1)}=x^{0}-\alpha z\\
由于g(x^{(1)})-g(x^{(0)})<TOL\\
答案是x^{(1)}=(0.48207,0.22485,0.93689)
$$
b.
$$
f_1(x_1,x_2,x_3)=10x_1-2x_2^2+x_2-2x_3-5\\
f_2(x_1,x_2,x_3)=8x_2^2+x_3^2-9\\
f_3(x_1,x_2,x_3)=8x_2x_3+4\\
x^{(0)}=0\\
F(x^{(0)})=(-5,-9,4)^t\\
J(x^{(0)}) = 
[\begin{matrix}
10&1&-2\\
0&0&0\\
0&0&0
\end{matrix}]\\
g(x)=f_1(x_1,x_2,x_3)^2+f_2(x_1,x_2,x_3)^2+f_3(x_1,x_2,x_3)^2\\
g(x^{(0)})=122\\
\nabla g(x)=2J(x)^tF(x)\\
\nabla g(x^{(0)})=
[\begin{matrix}
-100\\
-18\\
-16
\end{matrix}]\\
z_0=||\nabla g(x^{(0)})||_2=102.859127\\
z=\frac{1}{z_0}\nabla g(x^{0})=(-0.9722034681,-0.1749966243,-0.1555525549)^t\\
取\alpha_1=0\\
g_1=g(x^{(0)}-\alpha_1z)=g(x^{(0)})=122\\
取\alpha_3=1\\
g_3=g(x^{(0)}-\alpha_3z)=114.48938766804345\\
取\alpha_2=\alpha_3/2\\
g_2=g(x^{(0)}-\alpha_2z)=96.2811284177945\\
Set~P(\alpha)=g_1+h_1\alpha+h_3\alpha(\alpha-\alpha_2)\\
h_1=(g_2-g_1)/\alpha_2\\
h_2=(g_3-g_2)/(\alpha_3-\alpha_2)\\
h_3=(h_2-h_1)/\alpha_3\\
由于要找到\alpha 使得P最小，求导\\
P'(\alpha)=0\\
=>\alpha=0.3955950485\\
x^{(1)}=x^{0}-\alpha z\\
由于g(x^{(1)})-g(x^{(0)})<TOL\\
答案是x^{(1)}=(0.3845988781148877,0.06922779807729477,0.06153582049996441)
$$
