# HW 10

### 4-1

(1):
$$
T = 6\\
a_k = \frac{1}{N}\sum_{n=<N>}x[n]e^{-jk(\frac{2\pi}{N})n}\\
a_k = \frac{1}{6}(\sum_{k=0}^4e^{-jk(\frac{2\pi}{6})n})\\
a_k = \frac{1}{6}(cos\frac{\pi k}{3}+cos\frac{2\pi k}{3}-j(sin\frac{\pi k}{3}+sin\frac{2\pi  k}{3}))\\
|a_k| = \frac{1}{3}|cos\frac{k}{2}\pi+cos\frac{k}{6}\pi|\\
\theta = -\frac{\pi}{2}
$$
(3):$x[n] = \sum_{m=-∞}^∞\{2\delta[n-4m]+4\delta[n-1-4m]\}$
$$
T = 4\\
a_k = \frac{1}{N}\sum_{n=<N>}x[n]e^{-jk(\frac{2\pi}{N})n}\\
 = \frac{1}{4}(2+4e^{-jk(\frac{2\pi}{N})})\\
 a_k = \frac{1}{4}(2+4e^{-jk(\frac{\pi}{2})}) = \frac{1}{4}(2+4cosk\frac{\pi}{2}-4jsink\frac{\pi}{2})\\
 |a_k| = \sqrt{(\frac{1}{2}+cosk\frac{\pi}{2})^2+(sink\frac{\pi}{2})^2}\\
 相位:\theta = arctan(\frac{-sink\frac{\pi}{2}}{\frac{1}{2}+cosk\frac{\pi}{2}})\\
$$
(5)$x[n] = 1-sin(\pi n/4),n\in[0,3],x[n]以4为周期$
$$
T = 4,a_k = \frac{1}{N}\sum_{n=<N>}x[n]e^{-jk(\frac{2\pi}{N})n}\\
a_k = \frac{1}{4}(1+(1-\frac{1}{\sqrt2})e^{-j\frac{\pi}{2}}+(1+\frac{1}{\sqrt2})e^{-j\frac{3\pi}{2}})\\
 = \frac{1}{4}(1+(2-\sqrt2)cos(\frac{k\pi}{2}))\\
 |a_k| = |\frac{1}{4}(1+(2-\sqrt2)cos(\frac{k\pi}{2}))|\\
 \theta = 0
$$

### 4-2

(1)
$$
a_k = cos(\frac{k}{4}\pi)+sin(\frac{3k\pi}{4}),T = 8\\
a_k = \frac{1}{N}\sum_{n=<N>}x[n]e^{-jk(\frac{2\pi}{N})n}\\
a_k = \frac{1}{8}\sum x[n](cos(\frac{\pi}{4}kn)-jsin(\frac{\pi}{4}kn))\\
x[-3] = 4j,x[-1] = 4,x[1] = 4,x[3] = -4j,其余x[n] = 0
$$
(3)
$$
当n≠-2,2时,a_k = 1;n = -2或2时,a_k = 0\\
x[n] = \sum_{k=-3}^4a_ke^{jn(\frac{2\pi}{N})k}\\
 = 2+2cos\frac{n\pi}{2}+2cos\frac{3}{2}n\pi
$$
(5)
$$
a_k = -a_{k-4},x[2n+1] = (-1)^n\\
x[2n] = \sum_{k=<8>} a_ke^{jk\frac{\pi}{4}2n} = 0\\
x[2n] = 0,x[2n+1] = (-1)^n
$$

### 4-3

(1)
$$
x[n] = -x[n+\frac{N}{2}],证明a_{2k} = 0\\
a_{2k} = \frac{1}{N}\sum_{n=<N>}x[n]e^{-j2k(\frac{2\pi}{N})n}\\
由于x[n] = -x[n+\frac{N}{2}]\\
e^{-j2k(\frac{2\pi}{N})n} = e^{-j2k(\frac{2\pi}{N})(n+\frac{N}{2})}\\
a_{2k} = 0
$$
(2)
$$
N\%4 = 0,x[n] = -x[n+\frac{N}{4}]\\
a_{4k} = \frac{1}{N}\sum_{n=<N>}x[n]e^{-j4k(\frac{2\pi}{N})n}\\
由于x[n] = -x[n+\frac{N}{4}]\\
e^{-j4k(\frac{2\pi}{N})n} = e^{-j4k(\frac{2\pi}{N})(n+\frac{N}{4})}\\
a_{4k} = 0
$$

### 4-4

(1)
$$
a_k = b_k+jc_k\\
证明a_{-k} = a^*_k\\
x[n]<-^{FS}->a_k\\
x^*[n]<-^{FS}->a_{-k}^*\\
a_{-k}^* = a_k\\
a_{-k} = a_k^*\\
b_{-k}+jc_{-k} = b_{k}-jc_{k}\\
b_{k} = b_{-k},c_{-k} = -c_{k}
$$
(2)
$$
N为偶数,证明c_{N/2}=0,a_{N/2}是实数\\
a_{\frac{N}{2}} = \frac{1}{N}\sum_{n=<N>}x[n]e^{-j\frac{N}{2}(\frac{2\pi}{N})n}\\
 = \frac{1}{N}\sum x[n]e^{-j\pi n}\\
  = \frac{1}{N}\sum (-1)^nx[n]\\
  由于x[n]是实序列，a_{N/2}是实数，c_{N/2}=0
$$

